<?xml version='1.0' encoding='utf-8'?>

<section xml:id="session15-p2">
    <title>Session 15: Objectification of Properties, Part 2</title>
    <p>
      Okay, I spent a lot more time on Exercise 3 over the past week,
      but I think I'm starting to understand a little better.  If 
      I manage to make it through this problem this week, I'll take 
      that as a win!
    </p>
    <example>
        <title>Exercise 3: (continued)</title>
        
        
        <statement>
            <p>
                ...<em>evaluation at</em> 0 and <em>iteration</em>...
            </p>
        </statement>
        <solution>


    <p>
      I want to start this time by stepping back and look and assign
      some new names to the entities from the diagram I recreated last
      time.
    </p>
    <figure xml:id="fig-session15-ex3-2">
      <caption>Naming objects in "Iteration and evaluation defined"</caption>
      <image width="80%" xml:id="img-session15-ex3-2"> 
      <latex-image>
\begin{tikzpicture}[scale=.5]

\draw (-1,-2) rectangle (3,2);
\node (A) at (1,1) {Maps in $\mathcal{S}^{\circlearrowright}$};
\node (B) at (1,-1) {$\mathbb{N}^{\circlearrowright \sigma} \rightarrow Y^{\circlearrowright \beta}$};

\draw (8,-2) rectangle (12,2);
\node (C) at (10,1) {Maps in $\mathcal{S}$};
\node (D) at (10,-1) {$\mathbf{1} \rightarrow Y$};

\node (AS) at (1,2.5) {A};
\node (AS) at (10,2.5) {B};

\path[-{Stealth},font=\scriptsize,>=angle 90] 
($(A)+(2.5,0)$) edge node[above] {evaluation at 0 $= g$} ($(C)-(2.5,0)$)
($(D)-(2.5,0)$) edge node[below] {iteration $= h$} ($(B)+(2.5,0)$)
;

\end{tikzpicture}

      </latex-image>
      </image>
    </figure>
    <p>
        My reasoning here is that labeling my objects like this 
        will make it a little more clear on what exactly it would
        mean for our maps to be inverses.  Given the naming used
        above, I'd need to prove <m>h \circ g = 1_A</m> and 
        <m>g \circ h = 1_B</m>.  What makes this tricky is that 
        the objects in <m>A</m> are <m>\mathcal{S}^{\circlearrowright}</m>-maps
        that preserve the structure from
        <m>\boxed{\mathbb{N}^{\circlearrowright \sigma} \rightarrow Y^{\circlearrowright \beta}}</m>      
        and the objects in <m>B</m> are maps in <m>\mathcal{S}</m>
        from <m>\mathbf{1} \rightarrow Y</m> that don't necessarily 
        preserve any structure. 
    </p>
    <p>
        Perhaps what I should be doing is thinking of the maps
        <m>\mathbb{N}^{\circlearrowright \sigma} \xrightarrow{f} Y^{\circlearrowright \beta}</m>
        as a collection of arrows.  Each arrow needs to have a source point
        <m>n</m> in <m>\mathbb{N}</m> and a target point <m>y</m> in
        <m>Y</m>.  For <m>f</m> to preserve structure, we'd need to
        have <m>(f \circ \sigma)(n)= (\beta \circ f)(n)</m> for every
        <m>n</m> in <m>\mathbb{N}</m>.  
    </p>
    <p>
        Our map <m>g</m>, basically takes advantage of the fact that any map in
        <m>\mathbb{N}^{\circlearrowright \sigma} \xrightarrow{f} Y^{\circlearrowright \beta}</m>
        must be defined over the whole domain.  This means that there must be an 
        arrow originating at the point <m>0</m> pointing to some target point 
        <m>y = f 0</m> in <m>Y</m>.  We can then define <m>g: A \rightarrow B</m> such that
        for any <m>f \in A</m> we can define <m>g(f)</m> to be the map in 
        <m>\mathbf{1} \rightarrow Y</m> which maps the only element in <m>\mathbf{1}</m>
        to the point <m>f 0</m> in <m>Y</m>. 
    </p>
    <p>
        In contrast, our map <m>h</m> takes a map <m>\mathbf{1} \xrightarrow{y} Y</m> and uses it 
        to produce a map in <m>\mathbb{N}^{\circlearrowright \sigma} \xrightarrow{f} Y^{\circlearrowright \beta}</m>.
        It does this by applying <m>\beta</m> to <m>y</m> zero or more times, such that
        <m>f(n) = \beta^n(y)</m> for any <m>n \in \mathbb{N}</m>. 
        In the case where <m>n = 0</m>, the map <m>\beta</m> is never applied at all.  It follows that for 
        any <m>1 \xrightarrow{y} Y</m> in <m>B</m>, we're guaranteed to have
        <m>(g \circ h)(y) = g(h(y)) = g(f) = f 0 = \beta^0 y = y</m>. 
    </p>
    <p> 
        These two maps both produce maps, but handle structure differently.  The map <m>g</m>
        takes a map which preserves the structure and uses it to produce a map which might 
        not.  The map <m>h</m> takes a map which may not preserve structure and produces
        one that does.  The identity <m>(g \circ h)(y) = y</m> basically establishes that
        <m>g \circ h = 1_B</m> in <m>\mathcal{S}</m>, but I think we still need to establish
        that the map <m>h y</m> is valid in <m>\mathcal{S}^{\circlearrowright}</m>.
    </p>   
    <p>
        For any given <m>y</m>, the map <m>f = h \circ y</m> needs to satisfy 
        <m>(f \circ \sigma)(n) = (\beta \circ f)(n)</m> for every
        <m>n \in \mathbb{N}</m>.  
        At <m>n = 0</m>, <m>(f \circ \sigma)(0) = f \sigma 0 = f 1</m> and <m>(\beta \circ f)(0) = \beta f 0 = \beta y = f 1</m>.
        Since <m>(f \circ \sigma)(n) = (\beta \circ f)(n)</m> holds true for <m>n = 0</m>,
        we can use induction to establish that they must be the same for every 
        'successor'. 
    </p>
    <p> 
        Since each <m>n</m> can be represented as <m>n = \sigma^n 0</m>,
        we can use that to make a subsitution. 
        If follows that <m>(f \circ \sigma)(n) = (f \circ \sigma)(\sigma^n 0) = f \sigma \sigma^n 0 = f \sigma^{n+1} 0</m>
        and <m>(\beta \circ f)(n) = (\beta \circ f)(\sigma^n 0) = \beta f \sigma^n 0</m>.
        It also follows that <m>(f \circ \sigma)(n+1) = f \sigma^{n+2} 0</m>
        and <m>(\beta \circ f)(n+1) = \beta f \sigma^{n+1} 0</m>.  Since we know 
        that <m>f \sigma^{n+1} 0 = \beta f \sigma^n 0</m>, we can combine these
        two results to establish that
        <m>(\beta \circ f)(n+1) =  \beta f \sigma^{n+1} 0  = f \sigma \sigma^{n+1} 0 = f \sigma^{n+2} 0  = (f \circ \sigma)(n+1)</m>.
        Having established that <m>(f \circ \sigma)(0) = (\beta \circ f)(0)</m> and 
        <m>(f \circ \sigma)(n) = (\beta \circ f)(n) \implies (f \circ \sigma)(n+1) = (\beta \circ f)(n+1)</m>,
        <m>f \circ \sigma = \beta \circ f</m> follows by induction.
    </p>
    <p>
        Next, let's compose these maps in the reverse order to produce 
        the map <m>h \circ g: A \rightarrow A</m>.  Suppose we have some
        <m>\mathbb{N}^{\circlearrowright \sigma} \xrightarrow{f} Y^{\circlearrowright \beta}</m>
        in <m>A</m>.   It follows from our definitions that that        
        <m>(h \circ g)(f) = h(g(f)) = h(f 0) = h(y) = f</m> which would imply that 
        <m>h \circ g = 1_A</m>.  Having now established that both <m>h \circ g = 1_A</m>
        and <m>g \circ h = 1_B</m>, it's safe to refer to these two maps 
        as inverses.  
    </p>
    <p>
        Q.E.D.
    </p>
         </solution>
    </example>
</section>