<?xml version='1.0' encoding='utf-8'?>

<section xml:id="session27-p8">
    <title>Session 27: Examples of universal constructions, Part 8</title>
    <p>
        Let's keep pushing forward...
    </p>
    <example>
        <title>Exercise 5:</title>
        <statement>
            <p>
                If <m>B \xrightarrow{\alpha} A \xrightarrow{\beta} B</m>...

            </p>
        </statement>
        <solution>
            <p>
                We're given that <m>1_B = \beta \alpha</m> and 
                <m>f = \alpha \beta</m> is idempotent. Recall that
                <m>A \xrightarrow{f} A</m> is idempotent if and only if <m>f f = f</m>.
                This fact follows from associative and identity properties:
                <me>f f = (\alpha \beta) (\alpha \beta) = \alpha (\beta \alpha) \beta
                    = \alpha 1_B \beta = \alpha \beta = f</me>.
            </p>
            <p>
                We're asked to prove that <m>\alpha</m> is an 
                <em>equalizer</em> for the pair <m>f, 1_A</m>.  
                Per the definition, <m>B \xrightarrow{\alpha} A</m>
                is an equalizer of <m>f, 1_A</m> if 
                <m>f \alpha = 1_A \alpha</m> and for each 
                <m>T \xrightarrow{x} A</m> for which <m>f x = 1_A x</m>,
                there is exactly one <m>T \xrightarrow{e} B</m> for 
                which <m>x = \alpha e</m>.
            </p>
            <p>
                Let's start by demonstrating that <m>f \alpha = 1_A \alpha</m>.
            
            </p>
            <p>
                Given that <m>f = \alpha \beta</m>, we can precompose by
                <m>\alpha</m> to get
                <m>f \alpha = (\alpha \beta) \alpha</m>.
                By the associative property, 
                <m>(\alpha \beta) \alpha = \alpha (\beta \alpha)</m>, and 
                <m>\beta \alpha = 1_B</m>.  Subsitute and rewrite the identity maps
                to get
                <m>f \alpha = \alpha 1_B = \alpha = 1_A \alpha</m>.  
            </p>
            <p>
                Step one: complete. Our next one look a little trickier.
            </p>
            <p>
                For every 
                <m>T \xrightarrow{x} A</m> for which
              <m>f x = 1_A x</m> (or simply <m>f x = x</m>), we need to prove there
                is exactly one map
                <m>T \xrightarrow{e} B</m> for which <m>x = \alpha e</m>.
            </p>
            <p>
                First, we need to demonstrate that some such <m>e</m>
                must exist, then prove that we can't have 
                more than one such map.
            </p>
            <p>
                It seems obvious that for any <m>T \xrightarrow{x} A</m>
                satisfying <m>f x = x</m>
                the existance 
                of some <m>T \xrightarrow{e} B</m> would be
                guaranteed by the composition <m>\beta x</m>.
                Clearly <m>T \xrightarrow{x} A \xrightarrow{\beta} B</m>
                has the appropriate domain and codomain. Given <m>e = \beta x</m>,
                it follows that we can postcompose both sides by 
                <m>\alpha</m> to show <m>\alpha e = \alpha \beta x = f x = x</m>.
                The only remaining part of the question is: why can't we have more than one such map?
            </p>
        <p>
            Suppose we have a second map <m>T \xrightarrow{e'} B</m> 
            satisfying <m>\alpha e' = x</m> for some <m>e' \neq e</m>.
            For us to have <m>e' \neq e</m> 
            we'd need to have 
            a point <m>\mathbf{1} \xrightarrow{t} T</m> such that
            <m>e' t \neq e t</m>.  However, there is precisely one 
            map <m>\mathbf{1} \rightarrow T</m> by the definition of 
            terminal objects and that map needs to be an isomorphism.
        </p>
        <p>
            Since we know <m>\alpha e' = \alpha e = x</m>, we can postcompose
            by <m>\beta</m> and apply <m>\beta \alpha = 1_B</m> to get <m>\beta \alpha e' = e'= \beta \alpha e = e = \beta x</m>
            This contradicts our assumption that <m>e' \neq e</m> and proves 
            <m>e</m> is unique.
        </p>
           
            <p>
                This feels a bit like a <q>vacuous truth</q>.  
               If there's no <m>T \xrightarrow{x} A</m> such that 
               <m>f x = x</m>, then it doesn't matter what the 
               conclusion of the conditional statement is. 
        
            </p>
        </solution>
    </example>
    <p>
        I feel like this is another week
        with another unsatisfactory answer.
        I'm left wondering if I was supposed to 
        invoke a sum or product somehow to ensure
        the uniqueness of my map.
    </p>

  
</section>